updates

intermediate/Veritas.Intermediate.Global.fst
@@ -1,7 +1,7 @@
 module Veritas.Intermediate.Global
 
 let verifiable_implies_prefix_verifiable
-  (#vcfg:_) (gl:verifiable_log vcfg) (i:nat{i <= Seq.length gl}):
+  (#vcfg:_) (gl:verifiable_log vcfg) (i:nat{i <= S.length gl}):
   Lemma (ensures (verifiable #vcfg (SA.prefix gl i))) = 
   let pgl = SA.prefix gl i in
   let aux (tid: SA.seq_index pgl):
@@ -12,28 +12,218 @@ let verifiable_implies_prefix_verifiable
   in
   ()
 
-let add_seq (#vcfg:_) (gl: verifiable_log vcfg): seq (ms_hashfn_dom) = admit()
+let rec add_seq_aux (#vcfg:_) (gl: verifiable_log vcfg): 
+  Tot (seq (ms_hashfn_dom))
+  (decreases (S.length gl)) = 
+  let p = S.length gl in
+  if p = 0 then S.empty #(ms_hashfn_dom)
+  else
+    let gl' = SA.prefix gl (p - 1) in
+    // verifiable_implies_prefix_verifiable gl (p - 1);
+    append (add_seq_aux gl') (IntT.blum_add_seq (thread_log gl (p - 1)))
+
+let add_seq (#vcfg:_) (gl: verifiable_log vcfg): seq (ms_hashfn_dom) = 
+  add_seq_aux gl
+
+let rec lemma_g_hadd_correct_aux #vcfg (gl: verifiable_log vcfg):
+  Lemma (ensures (hadd gl = ms_hashfn (add_seq gl)))
+        (decreases (S.length gl)) = 
+  let p = S.length gl in
+  let s = add_seq gl in
+  let h = hadd gl in
+  if p = 0 then
+    lemma_hashfn_empty()
+  else (
+    let gl' = SA.prefix gl (p - 1) in
+    let s' = add_seq gl' in
+    let h' = hadd gl' in
+    lemma_g_hadd_correct_aux gl';
+    assert(h' = ms_hashfn s');
+
+    let tl = thread_log gl (p - 1) in
+    let st = blum_add_seq tl in
+    let ht = IntT.hadd tl in
+    IntT.lemma_hadd_correct tl;
+    lemma_hashfn_agg s' st
+  )
 
 let lemma_g_hadd_correct (#vcfg:_) (gl: verifiable_log vcfg):
-  Lemma (ensures (hadd gl = ms_hashfn (add_seq gl))) = admit()
+  Lemma (ensures (hadd gl = ms_hashfn (add_seq gl))) = 
+  lemma_g_hadd_correct_aux gl
+
+
+#push-options "--z3rlimit_factor 3"
+
+let rec add_set_map_aux #vcfg (gl: verifiable_log vcfg) (ii: sseq_index gl {is_blum_add (indexss gl ii)}):
+  Tot (j: SA.seq_index (add_seq gl){S.index (add_seq gl) j = blum_add_elem (indexss gl ii)})
+  (decreases (S.length gl))  
+  = 
+  let (tid, i) = ii in
+  let p = S.length gl in
+  let gl' = SA.prefix gl (p - 1) in
+  let s' = add_seq gl' in
+  let tl = thread_log gl (p - 1) in
+
+  if tid = p - 1 then
+    S.length s' + (IntT.add_seq_map tl i)
+  else
+    add_set_map_aux gl' ii  
+
+#pop-options
 
 (* mapping from blum_add entries in verifier log to the index in add seq *)
 let add_set_map (#vcfg:_) (gl: verifiable_log vcfg) (ii: sseq_index gl {is_blum_add (indexss gl ii)}):
-  (j: SA.seq_index (add_seq gl){S.index (add_seq gl) j = blum_add_elem (indexss gl ii)}) = admit()
+  (j: SA.seq_index (add_seq gl){S.index (add_seq gl) j = blum_add_elem (indexss gl ii)}) = 
+  add_set_map_aux gl ii
+
+let rec add_set_map_inv_aux (#vcfg:_) (gl: verifiable_log vcfg) (j: SA.seq_index (add_seq gl)):
+  Tot (ii: sseq_index gl {is_blum_add (indexss gl ii) /\ 
+                      add_set_map gl ii = j})
+  (decreases (S.length gl)) = 
+  let p = S.length gl in
+  let gl' = SA.prefix gl (p - 1) in
+  let s' = add_seq gl' in
+  let tl = thread_log gl (p - 1) in
+
+  if j < S.length s' then
+    add_set_map_inv_aux gl' j
+  else
+    let j' = j - S.length s' in
+    let i = IntT.add_seq_inv_map tl j' in
+    (p - 1, i)
 
 (* inverse mapping from add_seq to the blum add entries in the verifier logs *)
 let add_set_map_inv (#vcfg:_) (gl: verifiable_log vcfg) (j: SA.seq_index (add_seq gl)):
   (ii: sseq_index gl {is_blum_add (indexss gl ii) /\ 
-                      add_set_map gl ii = j}) = admit()
-                      
+                      add_set_map gl ii = j}) = add_set_map_inv_aux gl j
+
+let rec lemma_add_set_map_inv_aux (#vcfg:_) (gl: verifiable_log vcfg) (ii: sseq_index gl {is_blum_add (indexss gl ii)}):
+  Lemma (ensures (add_set_map_inv gl (add_set_map gl ii) = ii))
+        (decreases (S.length gl)) = 
+  let (tid, i) = ii in
+  let p = S.length gl in
+  let gl' = SA.prefix gl (p - 1) in
+  let s' = add_seq gl' in
+  let tl = thread_log gl (p - 1) in
+
+  if tid = p - 1 then ()
+  else
+    lemma_add_set_map_inv_aux gl' ii
+
 let lemma_add_set_map_inv (#vcfg:_) (gl: verifiable_log vcfg) (ii: sseq_index gl {is_blum_add (indexss gl ii)}):
-  Lemma (ensures (add_set_map_inv gl (add_set_map gl ii) = ii)) = admit()
+  Lemma (ensures (add_set_map_inv gl (add_set_map gl ii) = ii)) = lemma_add_set_map_inv_aux gl ii
 
 (* a single sequence containing all the blum evicts *)
-let evict_seq (#vcfg:_) (gl: verifiable_log vcfg): seq ms_hashfn_dom = admit()
+let rec evict_seq_aux (#vcfg:_) (gl: verifiable_log vcfg): 
+  Tot (seq ms_hashfn_dom)
+  (decreases (S.length gl)) =
+  let p = S.length gl in
+  if p = 0 then S.empty #(ms_hashfn_dom)
+  else
+    let gl' = SA.prefix gl (p - 1) in
+    append (evict_seq_aux gl') (IntT.blum_evict_seq (thread_log gl (p - 1)))
 
+(* a single sequence containing all the blum evicts *)
+let evict_seq (#vcfg:_) (gl: verifiable_log vcfg): seq ms_hashfn_dom = 
+  evict_seq_aux gl
+
+let rec lemma_ghevict_correct_aux (#vcfg:_) (gl: verifiable_log vcfg):
+  Lemma (ensures (hevict gl = ms_hashfn (evict_seq gl)))
+        (decreases (S.length gl)) = 
+  let p = S.length gl in
+  let s = evict_seq gl in
+  let h = hevict gl in
+  if p = 0 then
+    lemma_hashfn_empty()
+  else (
+    let gl' = SA.prefix gl (p - 1) in
+    let s' = evict_seq gl' in
+    let h' = hevict gl' in
+    lemma_ghevict_correct_aux gl';
+    let tl = thread_log gl (p - 1) in
+    let st = IntT.blum_evict_seq tl in
+    let ht = IntT.hevict tl in
+    IntT.lemma_hevict_correct tl;
+    
+    lemma_hashfn_agg s' st
+  )
+        
 let lemma_ghevict_correct (#vcfg:_) (gl: verifiable_log vcfg):
-  Lemma (ensures (hevict gl = ms_hashfn (evict_seq gl))) = admit()
+  Lemma (ensures (hevict gl = ms_hashfn (evict_seq gl))) =
+  lemma_ghevict_correct_aux gl
+
+(* two indexes of a sequence s are different *)
+let diff_elem (#a:eqtype) (s:seq a) (i1: SA.seq_index s) (i2: SA.seq_index s) = 
+  S.index s i1 <> S.index s i2
+
+let uniq_prop (#a:eqtype) (s: seq a) =
+  forall (i1: SA.seq_index s). 
+  forall (i2: SA.seq_index s).
+  {:pattern diff_elem s i1 i2}
+  i1 <> i2 ==> diff_elem s i1 i2
+
+(* for some reason, fstar is unable to assert (diff_elem s i1 i2) for uniq_prop s without 
+ * this lemma *)
+let lemma_uniq_idx (#a:eqtype) (s: seq a) (i1 i2: SA.seq_index s):
+  Lemma (requires (uniq_prop s /\ i1 <> i2)) 
+        (ensures (diff_elem s i1 i2))
+        [SMTPat (diff_elem s i1 i2)] = () 
+
+let lemma_uniq_prop_tail (#a:eqtype) (s: seq a{S.length s > 0}):
+  Lemma (requires (uniq_prop s))
+        (ensures (uniq_prop (S.tail s))) = 
+  let s' = tail s in
+  let aux (i1 i2: SA.seq_index s'):
+    Lemma (ensures (i1 <> i2 ==> diff_elem s' i1 i2))
+          [SMTPat (diff_elem s' i1 i2)] = 
+    
+    assert(S.index s (1 + i1) = S.index s' i1);          
+    assert(S.index s (1 + i2) = S.index s' i2);
+    if i1 = i2 then ()
+    else (
+      assert(diff_elem s' i1 i2 = diff_elem s (1 + i1) (1 + i2));
+      ()
+    )
+  in
+  ()
+
+let some_elem (#a:eqtype) (s: seq a) (x: a{count x s >= 1}): 
+  Tot (i:SA.seq_index s{S.index s i = x}) = index_mem x s  
+
+let rec lemma_count_len (#a:eqtype) (s: seq a) (x: a):
+  Lemma (ensures (count x s <= S.length s)) 
+        (decreases (S.length s))
+        = 
+  let n = S.length s in
+  if n = 0 then ()
+  else 
+    lemma_count_len (tail s) x
+
+let rec lemma_uniq_prop_counts (#a:eqtype) (s: seq a) (x: a):
+  Lemma (requires (uniq_prop s))
+        (ensures (count x s <= 1)) 
+        (decreases (S.length s)) = 
+  let n = S.length s in
+  if n <= 1 then lemma_count_len s x
+  else if count x s <= 1 then ()
+  else (
+    assert(uniq_prop s);
+    let h = head s in
+    let s' = tail s in
+
+    if h = x then (
+      assert(count x s' >= 1);
+      let i2 = some_elem s' x in
+      assert(S.index s (1 + i2) = x);
+      assert(diff_elem s 0 (1 + i2));
+      ()
+    )
+    else (
+      assert(count x s = count x s');
+      lemma_uniq_prop_tail s;
+      lemma_uniq_prop_counts s' x
+    )
+  )
 
 (* the global evict set is a set (not a multiset) *)
 let evict_set_is_set (#vcfg:_) (gl: verifiable_log vcfg): 
